theories/lr_lemmasTSel.v
@@ -9,65 +9,79 @@ Section Sec.
 
   Context (Γ: list ty).
 
+  (** Show that inclusion between postconditions is equivalent to inclusion
+      between value predicates *with an update modality. This is useful to show
+      equivalent value and expression subtyping, both for a fixed environment and
+      for environments matching a [Γ].
+   *)
+  Lemma inclusion_equiv_wp_upd {P Q}: ((□∀ e, WP e {{P}} → WP e {{Q}})%I ≡ (□∀ v, P v → |={⊤}=> Q v)%I).
+  Proof.
+    iSplit; iIntros "#Himpl !> * HP".
+    - setoid_rewrite wp_unfold.
+        by iApply ("Himpl" $! (of_val v)).
+    - iApply wp_fupd.
+      iApply (wp_wand with " [-]"); first iApply "HP".
+      iIntros "* HP". by iApply "Himpl".
+  Qed.
+
   Lemma mem_stp_sela_sub L U va l:
     ivtp Γ (TTMem l L U) va -∗
     Γ ⊨ L <: TSelA (pv va) l L U.
   Proof.
     iIntros "#Hva".
-    iApply istpEqIvstp.
-    (* cbn [interp uinterp interp_tmem]. *)
-    (* cbn [interp_tmem]. *)
-    (* unfold interp_tmem, defs_interp_tmem. *)
-    iIntros "/= !>" (v ρ) "#Hg #HvL".
+    rewrite istpEqIvstp.
+
+    iIntros "/= !> * Hg #HvL".
     iDestruct ("Hva" $! ρ with "Hg") as (ds) "#[% #H]"; iClear "Hva".
     iDestruct "H" as (φ σ) "#[Hl [#HLφ [#HφU #HLU]]]".
     simplOpen ds'; simpl.
     iExists (vobj ds'), σ, φ, ds.
-    (* TODO: prove a variant of istpEqIvstp, but one that is applicable here. *)
-  Admitted.
-  (*   repeat iModIntro. *)
-  (*   repeat iSplit; trivial. *)
-  (*   - iApply "HLU"; iApply "HvL". *)
-  (*   - *)
-  (*     (* Either *) *)
-  (*     (* by iLeft. *) *)
-  (*     (* Or *) *)
-  (*     iRight; iApply "HLφ"; iApply "HvL". *)
-  (* Qed. *)
+
+    iDestruct ("HLφ" with "HvL") as ">#HLφ'".
+    iDestruct ("HLU" with "HvL") as "> #HLU'".
+    (* iDestruct ("HφU" with "HLφ'") as "> #HφU1". *)
+    repeat iModIntro; repeat iSplit; trivial. by iRight.
+  Qed.
 
   Lemma mem_stp_sel_sub L U va l:
     ivtp Γ (TTMem l L U) va -∗
-    ivstp Γ (TLater L) (TSel (pv va) l).
+    uvstp Γ (TLater L) (TSel (pv va) l).
   Proof.
-    iIntros "/= #Hva !>" (v ρ) "#Hg #HvL !>".
+    iIntros "/= #Hva !> * #Hg #HvL".
     iDestruct ("Hva" $! ρ with "Hg") as (ds) "#[% #H]"; iClear "Hva".
     iDestruct "H" as (φ σ) "#[Hl [#HLφ [#HφU #HLU]]]".
     simplOpen ds'; simpl.
     iExists (vobj ds'), σ , φ, ds.
-    repeat iSplit; trivial.
-  Admitted.
-  (*   iRight; iApply "HLφ". iApply "HvL". *)
-  (* Qed. *)
+    iDestruct ("HLφ" with "HvL") as ">#HLφ'".
+    repeat iModIntro; repeat iSplit; trivial. by iRight.
+  Qed.
 
   Lemma mem_stp_sub_sel L U va l:
     ivtp Γ (TTMem l L U) va -∗
-    ivstp Γ (TSel (pv va) l) (TLater U).
+    uvstp Γ (TSel (pv va) l) (TLater U).
   Proof.
-    iIntros "/= #Hva !>" (v ρ) "#Hg #Hφ".
+    iIntros "/= #Hva !> * #Hg #Hφ".
     iDestruct ("Hva" $! ρ with "Hg") as (ds) "#[% #H]"; iClear "Hva".
     iDestruct "H" as (φ σ) "#[Hlφ [HLφ [HφU #HLU]]]".
     iDestruct "Hlφ" as (γ) "[% Hγφ]".
-  Admitted.
 
-  (*   iApply "HφU". *)
-  (*   simplOpen ds'; simpl. *)
-  (*   iDestruct "Hφ" as (va1 σ1 φ1 ds1) "[% [% [Hlφ1 [_ [[] | Hφ1v]]]]] /=". *)
-  (*   iDestruct "Hlφ1" as (γ1) "[% Hγφ1]". *)
+    iApply "HφU".
+    simplOpen ds'; simpl.
+    iDestruct "Hφ" as (va1 σ1 φ1 ds1) "[% [% [Hlφ1 [_ [[] | #Hφ1v]]]]] /=".
+    iDestruct "Hlφ1" as (γ1) "[% Hγφ1]".
 
-  (*   injectHyps; openDet; optFuncs_det. *)
+    injectHyps; openDet; optFuncs_det.
 
-  (*   iAssert (▷ (subst_phi σ ρ φ v ≡ subst_phi σ ρ φ1 v))%I as "#Hag"; simpl. *)
-  (*   { by iApply saved_pred_agree. } *)
-  (*   iNext; by iRewrite "Hag". *)
-  (* Qed. *)
+    iAssert (∀ ρ v, ▷ (φ (ρ, v) ≡ φ1 (ρ, v)))%I as "#Hag".
+      by iIntros; iApply saved_pred_agree.
+    (* iAssert (▷ (subst_phi σ ρ φ v ≡ subst_phi σ ρ φ1 v))%I as "#Hag"; simpl. *)
+    (*  ▷ (subst_phi σ ρ φ v ≡ subst_phi σ ρ φ1 v))%I as "#Hag". simpl. *)
+    (* { qy iApply saved_pred_agree. } *)
+    repeat iModIntro.
+    by iRewrite ("Hag" $! (vls_to_list σ.[to_subst ρ]) v).
+  Qed.
+
+    (* iDestruct ("HLφ" with "HvL") as ">#HLφ'". *)
+    (* iDestruct ("HLU" with "HvL") as "> #HLU'". *)
+    (* iDestruct ("HφU" with "HLφ'") as "> #HφU1". *)
 End Sec.
